

Laplace Transforms

Following chapter 4 in CLP3.

Ex 4.1.3.

$$\frac{d^2 y}{dt^2} = 0.$$

Solve this subject to the boundary conditions $y(0)=1$, $y(1)=2$.

Solution

$$\frac{d^2 y}{dt^2} = 0$$

$$\Rightarrow \frac{dy}{dt} = c, \text{ a constant.}$$

$$\Rightarrow y(t) = ct + d, \text{ } d \text{ a constant.}$$

the parameters c, d are determined by given boundary conditions

$$y(0) = 1 \Rightarrow c \cdot 0 + d = 1 \Rightarrow d = 1$$

$$y(1) = 2 \Rightarrow c \cdot 1 + 1 = 2 \Rightarrow c = 1$$

So the unique solution
is $y(t) = t + 1$.

Some general remarks about the
concept of "transforming" problems.

Hard problems in one domain
might be transformed to easier
problems in another domain. ~~XXXX~~

Solve the problem there
then apply an inverse transform
to recover the solution to the
original.

Eg. Arithmetic computations

Hard

$$a^b$$

log →

Easier

$$\log(a^b) = b \cdot \log(a)$$

$$ab$$

$$\log(ab) = \log(a) + \log(b)$$

←
exp.

Def Laplace transform

$$\mathcal{L}\{f(t)\} = \int_0^{\infty} e^{-\underline{s}t} f(t) dt.$$

function of the
new variable s .

other notations.

$$\mathcal{L}\{f(t)\} = F(s) = \overline{f}(s)$$

Another 'transform' you might recall

Power series / Taylor series.

(\hookrightarrow) takes an ^{infinite} sequence of coefficients a_0, a_1, a_2, \dots

and builds an associated function.

$$A(x) = \sum_{i=0}^{\infty} a_i x^i$$

Can view a sequence a_0, a_1, a_2, \dots as a function $f: \mathbb{N}^{\geq 0} \rightarrow \mathbb{R}$.

$$\mathcal{L}\{f(t)\} = \int_0^{\infty} e^{-st} f(t) dt.$$

$(e^{-s})^t$

Can regard the Laplace transform as "kind of" a continuous version of the power series transform.

Ex 4.2.2 Consider the constant function f , defined by

$$f(t) = 1, \text{ for } t \geq 0.$$

$$\mathcal{L}\{f(t)\} = \mathcal{L}\{1\}$$

$$= \int_0^{\infty} e^{-st} dt$$

$$= \left[\frac{e^{-st}}{-s} \right]_0^{\infty}.$$

$$= \frac{2}{s^3}$$

keep repeating this for $\mathcal{L}\{t^3\}, \mathcal{L}\{t^4\}, \dots$
to get

$$\mathcal{L}\{t^n\} = \frac{n!}{s^{n+1}}$$

Corollary 4.4.6.

$$\mathcal{L}\left\{\frac{d^2x}{dt^2}\right\} = \mathcal{L}\left\{\frac{d}{dt}\left(\frac{dx}{dt}\right)\right\}$$

$$= s \mathcal{L}\left\{\frac{dx}{dt}\right\} - \left.\frac{dx}{dt}\right|_{t=0}$$

$$= s \left(s \mathcal{L}\{x(t)\} - x(0) \right)$$

$$- \left.\frac{dx}{dt}\right|_{t=0}$$

$$= s^2 \mathcal{L}\{x(t)\} - s x(0) - \left.\frac{dx}{dt}\right|_{t=0}.$$

keep applying this to get Cor 4.4.6.

Put in initial conditions.

$$s^2 \bar{y} - 5s\bar{y} + 4\bar{y} = \frac{12}{s}$$

$$(s^2 - 5s + 4) \bar{y} = \frac{12}{s}$$

$$\Rightarrow \bar{y}(s) = \frac{12}{s(s^2 - 5s + 4)} \quad \textcircled{\otimes}$$

$$\Rightarrow y(t) = \mathcal{L}^{-1} \{ \bar{y} \}$$

$$= \mathcal{L}^{-1} \left\{ \frac{12}{s(s^2 - 5s + 4)} \right\}$$

$$= ?$$

In order to use results from table we first need to expand \bar{y} into its partial fraction expansion.

$$\bar{y} = \frac{12}{s(s-4)(s-1)}$$

$$= \frac{\alpha}{s} + \frac{\beta}{s-4} + \frac{\gamma}{s-1}$$

by
partial
fractions

